$$
\begin{align*}
\min_{h} \; L &= \frac{1}{\Delta l}\sum\limits_{i=1}^{256} \sum\limits_{j=1}^{256}  \sqrt{(\Delta l)^2 + [h(i+1, j) - h(i, j)]^2 + [h(i,j+1) - h(i,j)]^2} \\
& \quad + c \cdot \sum\limits_{(i, j) \in \mathcal{I}} (h(i,j) - v(i, j))^2 - \lambda \cdot \sum\limits_{(i, j) \in \mathcal{I}} (h(i,j) - v(i, j)) \\
\nabla_{i,j} L &= \frac{2}{\Delta l} \left\{ \frac{2h(i, j) - h(i+1, j) - h(i,j+1)}{\sqrt{(\Delta l)^2 + [h(i+1, j) - h(i, j)]^2 + [h(i,j+1) - h(i,j)]^2}} + \\ 
     \frac{h(i, j) - h(i-1, j)}{\sqrt{(\Delta l)^2 + [h(i, j) - h(i-1, j)]^2 + [h(i-1,j+1) - h(i-1,j)]^2}} \\
      \frac{h(i, j) - h(i,j-1)}{\sqrt{(\Delta l)^2 + [h(i+1, j-1) - h(i, j-1)]^2 + [h(i,j) - h(i,j-1)]^2}} \right\}
\end{align*}
$$



if i == M and j < M:
$$
\begin{align*}
L &= \frac{1}{\Delta l}\sum\limits_{i=1}^{256} \sum\limits_{j=1}^{256}  \sqrt{(\Delta l)^2 + [h(i, j) - h(i-1, j)]^2 + [h(i,j+1) - h(i,j)]^2} \\
\nabla_{i,j} L &= \frac{2}{\Delta l} \left\{ \frac{2h(i, j) - h(i-1, j) - h(i,j+1)}{\sqrt{(\Delta l)^2 + [h(i-1, j) - h(i, j)]^2 + [h(i,j+1) - h(i,j)]^2}} + \\ 
     \frac{h(i, j) - h(i-1, j)}{\sqrt{(\Delta l)^2 + [h(i, j) - h(i-1, j)]^2 + [h(i-1,j+1) - h(i-1,j)]^2}} \\
      \frac{h(i, j) - h(i,j-1)}{\sqrt{(\Delta l)^2 + [h(i+1, j-1) - h(i, j-1)]^2 + [h(i,j) - h(i,j-1)]^2}} \right\}
\end{align*}
$$
